HOLean/Elab.lean
@@ -5,4 +5,5 @@ Released under Apache 2.0 license as described in the file LICENSE.
 
 import HOLean.Elab.Translate
 import HOLean.Elab.Term
+import HOLean.Elab.Command
 import HOLean.Elab.Tests
